Iris/Iris/BI/WeakestPre.lean
@@ -1,10 +1,21 @@
 module
 
 public import Iris.Std.CoPset
+public import Iris.BI
+public meta import Iris.BI
+public import Iris.BI.BIBase
 public meta import Iris.Std.Rewrite
 public import Std
 meta import Lean
 public import Lean
+
+public import Iris.BI.BI
+public import Iris.BI.Classes
+public import Iris.BI.DerivedLaws
+public import Iris.BI.DerivedLawsLater
+public import Iris.BI.Extensions
+public import Iris.BI.SIProp
+public meta import Iris.Std.RocqPorting
 
 public section
 
@@ -39,17 +50,21 @@ class TotalWP (PROP Expr) (Val : outParam (Type _)) (A : Type _) where
 syntax wp_expr :=
     term:max (" @ " term:max (" ; " term:max) <|> ((" ? ")? )) <|> (" ? ")?
 
-declare_syntax_cat wp_postcond_inner
-syntax ident ", " term : wp_postcond_inner
-syntax term : wp_postcond_inner
+declare_syntax_cat wpPostcondInner
+syntax ident ", " term : wpPostcondInner
+syntax term : wpPostcondInner
 
-declare_syntax_cat wp_postcond
-syntax " {{ " wp_postcond_inner " }} " : wp_postcond
-syntax " [{ " wp_postcond_inner " }] " : wp_postcond
-syntax " ⦃ " wp_postcond_inner " ⦄ " : wp_postcond -- Are spaces outside of parens used in the pp?
-syntax " 〖 " wp_postcond_inner " 〗 "  : wp_postcond
+declare_syntax_cat wpPostcond
+syntax " {{ " wpPostcondInner " }} " : wpPostcond
+syntax " [{ " wpPostcondInner " }] " : wpPostcond
+syntax " ⦃ " wpPostcondInner " ⦄ " : wpPostcond -- Are spaces outside of parens used in the pp?
+syntax " 〖 " wpPostcondInner " 〗 "  : wpPostcond
 
-syntax (name := wp) "WP " wp_expr wp_postcond : term
+syntax (name := wp) "WP " wp_expr wpPostcond : term
+
+syntax texanPostcond := (ident+ ", ")? " RET " term:min "; " term
+
+syntax (name := texanTriple) "{{{ " term " }}} " wp_expr " {{{ " texanPostcond " }}}" : term
 
 /- This section checks whether the syntax is recognized correctly for all combinations -/
 section testNotation
@@ -64,53 +79,264 @@ elab "#no_info" "in" cmd:command : command => do
     }
   }
 
-#no_info in #check_failure WP e @ s ; E {{ Φ }}
-#no_info in #check_failure WP e @ E {{ Φ }}
-#no_info in #check_failure WP e @ E ? {{ Φ }}
-#no_info in #check_failure WP e {{ Φ }}
-#no_info in #check_failure WP e ? {{ Φ }}
+/--
+info: elaboration function for `wp` has not been implemented
+  WP e @ s ; E {{ Φ }}
+-/
+#guard_msgs in #check_failure WP e @ s ; E {{ Φ }}
+/--
+info: elaboration function for `wp` has not been implemented
+  WP e @ E {{ Φ }}
+-/
+#guard_msgs in #check_failure WP e @ E {{ Φ }}
+/--
+info: elaboration function for `wp` has not been implemented
+  WP e @ E ? {{ Φ }}
+-/
+#guard_msgs in #check_failure WP e @ E ? {{ Φ }}
+/--
+info: elaboration function for `wp` has not been implemented
+  WP e {{ Φ }}
+-/
+#guard_msgs in #check_failure WP e {{ Φ }}
+/--
+info: elaboration function for `wp` has not been implemented
+  WP e ? {{ Φ }}
+-/
+#guard_msgs in #check_failure WP e ? {{ Φ }}
 
-#no_info in #check_failure WP e @ s ; E {{v,  Φ }}
-#no_info in #check_failure WP e @ E {{v,  Φ }}
-#no_info in #check_failure WP e @ E ? {{v,  Φ }}
-#no_info in #check_failure WP e {{v,  Φ }}
-#no_info in #check_failure WP e ? {{v,  Φ }}
+/--
+info: elaboration function for `wp` has not been implemented
+  WP e @ s ; E {{ v, Φ }}
+-/
+#guard_msgs in #check_failure WP e @ s ; E {{v,  Φ }}
+/--
+info: elaboration function for `wp` has not been implemented
+  WP e @ E {{ v, Φ }}
+-/
+#guard_msgs in #check_failure WP e @ E {{v,  Φ }}
+/--
+info: elaboration function for `wp` has not been implemented
+  WP e @ E ? {{ v, Φ }}
+-/
+#guard_msgs in #check_failure WP e @ E ? {{v,  Φ }}
+/--
+info: elaboration function for `wp` has not been implemented
+  WP e {{ v, Φ }}
+-/
+#guard_msgs in #check_failure WP e {{v,  Φ }}
+/--
+info: elaboration function for `wp` has not been implemented
+  WP e ? {{ v, Φ }}
+-/
+#guard_msgs in #check_failure WP e ? {{v,  Φ }}
 
-#no_info in #check_failure WP e @ s ; E ⦃ Φ ⦄
-#no_info in #check_failure WP e @ E ⦃ Φ ⦄
-#no_info in #check_failure WP e @ E ? ⦃ Φ ⦄
-#no_info in #check_failure WP e ⦃ Φ ⦄
-#no_info in #check_failure WP e ? ⦃ Φ ⦄
+/--
+info: elaboration function for `wp` has not been implemented
+  WP e @ s ; E ⦃ Φ ⦄
+-/
+#guard_msgs in #check_failure WP e @ s ; E ⦃ Φ ⦄
+/--
+info: elaboration function for `wp` has not been implemented
+  WP e @ E ⦃ Φ ⦄
+-/
+#guard_msgs in #check_failure WP e @ E ⦃ Φ ⦄
+/--
+info: elaboration function for `wp` has not been implemented
+  WP e @ E ? ⦃ Φ ⦄
+-/
+#guard_msgs in #check_failure WP e @ E ? ⦃ Φ ⦄
+/--
+info: elaboration function for `wp` has not been implemented
+  WP e ⦃ Φ ⦄
+-/
+#guard_msgs in #check_failure WP e ⦃ Φ ⦄
+/--
+info: elaboration function for `wp` has not been implemented
+  WP e ? ⦃ Φ ⦄
+-/
+#guard_msgs in #check_failure WP e ? ⦃ Φ ⦄
 
-#no_info in #check_failure WP e @ s ; E ⦃v,  Φ ⦄
-#no_info in #check_failure WP e @ E ⦃v,  Φ ⦄
-#no_info in #check_failure WP e @ E ? ⦃v,  Φ ⦄
-#no_info in #check_failure WP e ⦃v,  Φ ⦄
-#no_info in #check_failure WP e ? ⦃v,  Φ ⦄
+/--
+info: elaboration function for `wp` has not been implemented
+  WP e @ s ; E ⦃ v, Φ ⦄
+-/
+#guard_msgs in #check_failure WP e @ s ; E ⦃v,  Φ ⦄
+/--
+info: elaboration function for `wp` has not been implemented
+  WP e @ E ⦃ v, Φ ⦄
+-/
+#guard_msgs in #check_failure WP e @ E ⦃v,  Φ ⦄
+/--
+info: elaboration function for `wp` has not been implemented
+  WP e @ E ? ⦃ v, Φ ⦄
+-/
+#guard_msgs in #check_failure WP e @ E ? ⦃v,  Φ ⦄
+/--
+info: elaboration function for `wp` has not been implemented
+  WP e ⦃ v, Φ ⦄
+-/
+#guard_msgs in #check_failure WP e ⦃v,  Φ ⦄
+/--
+info: elaboration function for `wp` has not been implemented
+  WP e ? ⦃ v, Φ ⦄
+-/
+#guard_msgs in #check_failure WP e ? ⦃v,  Φ ⦄
 
-#no_info in #check_failure WP e @ s ; E [{ Φ }]
-#no_info in #check_failure WP e @ E [{ Φ }]
-#no_info in #check_failure WP e @ E ? [{ Φ }]
-#no_info in #check_failure WP e [{ Φ }]
-#no_info in #check_failure WP e ? [{ Φ }]
+/--
+info: elaboration function for `wp` has not been implemented
+  WP e @ s ; E [{ Φ }]
+-/
+#guard_msgs in #check_failure WP e @ s ; E [{ Φ }]
+/--
+info: elaboration function for `wp` has not been implemented
+  WP e @ E [{ Φ }]
+-/
+#guard_msgs in #check_failure WP e @ E [{ Φ }]
+/--
+info: elaboration function for `wp` has not been implemented
+  WP e @ E ? [{ Φ }]
+-/
+#guard_msgs in #check_failure WP e @ E ? [{ Φ }]
+/--
+info: elaboration function for `wp` has not been implemented
+  WP e [{ Φ }]
+-/
+#guard_msgs in #check_failure WP e [{ Φ }]
+/--
+info: elaboration function for `wp` has not been implemented
+  WP e ? [{ Φ }]
+-/
+#guard_msgs in #check_failure WP e ? [{ Φ }]
 
-#no_info in #check_failure WP e @ s ; E [{v,  Φ }]
-#no_info in #check_failure WP e @ E [{v,  Φ }]
-#no_info in #check_failure WP e @ E ? [{v,  Φ }]
-#no_info in #check_failure WP e [{v,  Φ }]
-#no_info in #check_failure WP e ? [{v,  Φ }]
+/--
+info: elaboration function for `wp` has not been implemented
+  WP e @ s ; E [{ v, Φ }]
+-/
+#guard_msgs in #check_failure WP e @ s ; E [{v,  Φ }]
+/--
+info: elaboration function for `wp` has not been implemented
+  WP e @ E [{ v, Φ }]
+-/
+#guard_msgs in #check_failure WP e @ E [{v,  Φ }]
+/--
+info: elaboration function for `wp` has not been implemented
+  WP e @ E ? [{ v, Φ }]
+-/
+#guard_msgs in #check_failure WP e @ E ? [{v,  Φ }]
+/--
+info: elaboration function for `wp` has not been implemented
+  WP e [{ v, Φ }]
+-/
+#guard_msgs in #check_failure WP e [{v,  Φ }]
+/--
+info: elaboration function for `wp` has not been implemented
+  WP e ? [{ v, Φ }]
+-/
+#guard_msgs in #check_failure WP e ? [{v,  Φ }]
 
-#no_info in #check_failure WP e @ s ; E 〖 Φ 〗
-#no_info in #check_failure WP e @ E 〖 Φ 〗
-#no_info in #check_failure WP e @ E ? 〖 Φ 〗
-#no_info in #check_failure WP e 〖 Φ 〗
-#no_info in #check_failure WP e ? 〖 Φ 〗
+/--
+info: elaboration function for `wp` has not been implemented
+  WP e @ s ; E 〖 Φ 〗
+-/
+#guard_msgs in #check_failure WP e @ s ; E 〖 Φ 〗
+/--
+info: elaboration function for `wp` has not been implemented
+  WP e @ E 〖 Φ 〗
+-/
+#guard_msgs in #check_failure WP e @ E 〖 Φ 〗
+/--
+info: elaboration function for `wp` has not been implemented
+  WP e @ E ? 〖 Φ 〗
+-/
+#guard_msgs in #check_failure WP e @ E ? 〖 Φ 〗
+/--
+info: elaboration function for `wp` has not been implemented
+  WP e 〖 Φ 〗
+-/
+#guard_msgs in #check_failure WP e 〖 Φ 〗
+/--
+info: elaboration function for `wp` has not been implemented
+  WP e ? 〖 Φ 〗
+-/
+#guard_msgs in #check_failure WP e ? 〖 Φ 〗
 
-#no_info in #check_failure WP e @ s ; E 〖v,  Φ 〗
-#no_info in #check_failure WP e @ E 〖v,  Φ 〗
-#no_info in #check_failure WP e @ E ? 〖v,  Φ 〗
-#no_info in #check_failure WP e 〖v,  Φ 〗
-#no_info in #check_failure WP e ? 〖v,  Φ 〗
+/--
+info: elaboration function for `wp` has not been implemented
+  WP e @ s ; E 〖 v, Φ 〗
+-/
+#guard_msgs in #check_failure WP e @ s ; E 〖v,  Φ 〗
+/--
+info: elaboration function for `wp` has not been implemented
+  WP e @ E 〖 v, Φ 〗
+-/
+#guard_msgs in #check_failure WP e @ E 〖v,  Φ 〗
+/--
+info: elaboration function for `wp` has not been implemented
+  WP e @ E ? 〖 v, Φ 〗
+-/
+#guard_msgs in #check_failure WP e @ E ? 〖v,  Φ 〗
+/--
+info: elaboration function for `wp` has not been implemented
+  WP e 〖 v, Φ 〗
+-/
+#guard_msgs in #check_failure WP e 〖v,  Φ 〗
+/--
+info: elaboration function for `wp` has not been implemented
+  WP e ? 〖 v, Φ 〗
+-/
+#guard_msgs in #check_failure WP e ? 〖v,  Φ 〗
+
+/--
+info: elaboration function for `texanTriple` has not been implemented
+  {{{ P }}} e @ s ; E {{{ x y, RET pat; Q }}}
+-/
+#guard_msgs in #check_failure {{{ P }}} e @ s ; E {{{ x y , RET pat ; Q }}}
+/--
+info: elaboration function for `texanTriple` has not been implemented
+  {{{ P }}} e @ E {{{ x y, RET pat; Q }}}
+-/
+#guard_msgs in #check_failure {{{ P }}} e @ E {{{ x y , RET pat ; Q }}}
+/--
+info: elaboration function for `texanTriple` has not been implemented
+  {{{ P }}} e @ E ? {{{ x y, RET pat; Q }}}
+-/
+#guard_msgs in #check_failure {{{ P }}} e @ E ? {{{ x y , RET pat ; Q }}}
+/--
+info: elaboration function for `texanTriple` has not been implemented
+  {{{ P }}} e {{{ x y, RET pat; Q }}}
+-/
+#guard_msgs in #check_failure {{{ P }}} e {{{ x y , RET pat ; Q }}}
+/--
+info: elaboration function for `texanTriple` has not been implemented
+  {{{ P }}} e ? {{{ x y, RET pat; Q }}}
+-/
+#guard_msgs in #check_failure {{{ P }}} e ? {{{ x y , RET pat ; Q }}}
+/--
+info: elaboration function for `texanTriple` has not been implemented
+  {{{ P }}} e @ s ; E {{{ RET pat; Q }}}
+-/
+#guard_msgs in #check_failure {{{ P }}} e @ s ; E {{{ RET pat ; Q }}}
+/--
+info: elaboration function for `texanTriple` has not been implemented
+  {{{ P }}} e @ E {{{ RET pat; Q }}}
+-/
+#guard_msgs in #check_failure {{{ P }}} e @ E {{{ RET pat ; Q }}}
+/--
+info: elaboration function for `texanTriple` has not been implemented
+  {{{ P }}} e @ E ? {{{ RET pat; Q }}}
+-/
+#guard_msgs in #check_failure {{{ P }}} e @ E ? {{{ RET pat ; Q }}}
+/--
+info: elaboration function for `texanTriple` has not been implemented
+  {{{ P }}} e {{{ RET pat; Q }}}
+-/
+#guard_msgs in #check_failure {{{ P }}} e {{{ RET pat ; Q }}}
+/--
+info: elaboration function for `texanTriple` has not been implemented
+  {{{ P }}} e ? {{{ RET pat; Q }}}
+-/
+#guard_msgs in #check_failure {{{ P }}} e ? {{{ RET pat ; Q }}}
 
 end testNotation
 
@@ -129,20 +355,20 @@ meta def parseWpExpr : Lean.TSyntax `wp_expr → Lean.MacroM (TSyntax `term × T
   | _ => Lean.Macro.throwUnsupported
 
 open Lean in
-meta def parseWpPostcondInner (stx : TSyntax `wp_postcond_inner) : MacroM (TSyntax `term) := do
+meta def parseWpPostcondInner (stx : TSyntax `wpPostcondInner) : MacroM (TSyntax `term) := do
   match stx with
-  | `(wp_postcond_inner| $v:ident, $Φ:term) => `(fun $v => $Φ)
-  | `(wp_postcond_inner| $Φ:term) => return Φ
+  | `(wpPostcondInner| $v:ident, $Φ:term) => `(fun $v => $Φ)
+  | `(wpPostcondInner| $Φ:term) => return Φ
   | _ => Macro.throwUnsupported
 
 open Lean in
-meta def parseWpPostcond (stx : TSyntax `wp_postcond) : MacroM (TSyntax `term × Bool) := do
+meta def parseWpPostcond (stx : TSyntax `wpPostcond) : MacroM (TSyntax `term × Bool) := do
   match stx with
-  | `(wp_postcond| {{ $inner:wp_postcond_inner }})
-  | `(wp_postcond| ⦃ $inner:wp_postcond_inner ⦄) =>
+  | `(wpPostcond| {{ $inner:wpPostcondInner }})
+  | `(wpPostcond| ⦃ $inner:wpPostcondInner ⦄) =>
     return (←parseWpPostcondInner inner, false)
-  | `(wp_postcond| [{ $inner:wp_postcond_inner }])
-  | `(wp_postcond| 〖 $inner:wp_postcond_inner 〗) =>
+  | `(wpPostcond| [{ $inner:wpPostcondInner }])
+  | `(wpPostcond| 〖 $inner:wpPostcondInner 〗) =>
     return (←parseWpPostcondInner inner, true)
   | _ => Macro.throwUnsupported (α := TSyntax `term × Bool)
 
@@ -158,10 +384,78 @@ meta def wpMacro : Lean.Macro := fun stx => do
       `(Wp.wp $s $E $e $Φ)
   | _ => Lean.Macro.throwUnsupported
 
+-- syntax (name := underExtraBinders) "underExtraBinders(" term:min ")" : term
+-- syntax (name := sourceExtraBinders) "sourceExtraBinders(" term ")" : term
+
+-- private meta partial def findSource : Syntax → Option Syntax
+-- | .missing => none
+-- | .node _ ``sourceExtraBinders args => do
+--   let #[_, inner, _] := args | none
+--   return inner
+-- | .node _ _ args => do
+--   let #[res] := args.filterMap findSource | none
+--   return res
+-- | .ident _ _ _ _ => none
+-- | .atom _ _ => none
+
+-- private meta partial def collectUnresolvedIds : Syntax → Elab.Term.TermElabM (Array Ident)
+-- | .missing => return {}
+-- | .node _ _ args => do
+--   args.flatMapM collectUnresolvedIds
+-- | id@(.ident ..) => do
+--   try
+--     let _ ← Elab.Term.elabIdent id .none
+--     return {}
+--   catch
+--   | .error _ md =>
+--     let msg ← md.toString
+--     if msg.startsWith "Unknown identifier" then
+--       return #[⟨id⟩]
+--     else
+--       return {}
+--   | _ => return {}
+-- | .atom _ _ =>
+--   return {}
+
+-- elab "sourceExtraBinders(" t:term ")" : term => Elab.Term.elabTerm t .none
+
+-- @[term_elab underExtraBinders]
+-- meta def elabUnderExtraBinders: Elab.Term.TermElab := fun stx ty? => do
+--   match stx with
+--   | `(underExtraBinders( $t:term ) ) =>
+--     if let .some s := findSource t then
+--       -- logInfo s!"Found! {s.getArgs.size} {repr s}"
+--       let ids ← collectUnresolvedIds s
+--       logInfo s!"Collected identifiers {ids}"
+--       let stx ← `(∀ $ids*, $t)
+--       Elab.Term.elabTerm stx ty?
+--     else
+--       Elab.Term.elabTerm t ty?
+--   | _ => unreachable!
+
+-- macro_rules
+-- | `(iprop(underExtraBinders($t))) => `(underExtraBinders(iprop($t)))
+-- | `(iprop(sourceExtraBinders($t))) => `(sourceExtraBinders(iprop($t)))
+
+-- @[macro texanTriple]
+-- meta def wpTexanTriple : Lean.Macro
+--   | `({{{ $P:term }}} $expr {{{ $[$[$xs:ident]* ,]? RET $pat ; $Q }}}) => do
+--     let xs : TSyntaxArray `ident := xs.getD #[]
+--     `(iprop(∀ Φ, $P -∗ ▷ (∀ $xs*, underExtraBinders($Q → Φ sourceExtraBinders($pat))) -∗ (WP $expr {{ Φ }})))
+--   | _ => Lean.Macro.throwUnsupported
+
+@[macro texanTriple]
+meta def wpTexanTriple : Lean.Macro
+  | `({{{ $P:term }}} $expr {{{ $[$[$xs:ident]* ,]? RET $pat ; $Q }}}) => do
+    let xs : TSyntaxArray `ident := xs.getD #[]
+    `(iprop(∀ Φ, $P -∗ ▷ (∀ $xs*, $Q → Φ $pat) -∗ (WP $expr {{ Φ }})))
+  | _ => Lean.Macro.throwUnsupported
+
 section testElab
 set_option linter.unusedVariables false
 
 variable (PROP Expr : Type _) (Val : outParam (Type _)) (A : Type _)
+variable [ι : Iris.BI PROP]
 variable [Wp PROP Expr Val A]
 variable [Wp PROP Expr Val Stuckness]
 variable [TotalWP PROP Expr Val A]
@@ -173,7 +467,7 @@ variable (Φ : PROP)
 /-- info: Wp.wp s E e fun v => Φ : PROP -/
 #guard_msgs in #check WP e @ s ; E {{v,  Φ }}
 /-- info: Wp.wp Stuckness.NotStuck E e fun v => Φ : PROP -/
-#guard_msgs in #check WP e @ E {{ v,  Φ}}
+#guard_msgs in #check WP e @ E {{ v, Φ }}
 /-- info: Wp.wp Stuckness.NotStuck ⊤ e fun v => Φ : PROP -/
 #guard_msgs in #check WP e {{v,  Φ }}
 /-- info: Wp.wp Stuckness.MaybeStuck ⊤ e fun v => Φ : PROP -/
@@ -182,7 +476,7 @@ variable (Φ : PROP)
 /-- info: TotalWP.totalWp s E e fun v => Φ : PROP -/
 #guard_msgs in #check WP e @ s ; E [{v,  Φ }]
 /-- info: TotalWP.totalWp Stuckness.NotStuck E e fun v => Φ : PROP -/
-#guard_msgs in #check WP e @ E [{ v,  Φ}]
+#guard_msgs in #check WP e @ E [{ v, Φ }]
 /-- info: TotalWP.totalWp Stuckness.NotStuck ⊤ e fun v => Φ : PROP -/
 #guard_msgs in #check WP e [{v,  Φ }]
 /-- info: TotalWP.totalWp Stuckness.MaybeStuck ⊤ e fun v => Φ : PROP -/
@@ -193,7 +487,7 @@ variable (Φ : Val → PROP)
 /-- info: Wp.wp s E e Φ : PROP -/
 #guard_msgs in #check WP e @ s ; E {{ Φ }}
 /-- info: Wp.wp Stuckness.NotStuck E e Φ : PROP -/
-#guard_msgs in #check WP e @ E {{  Φ}}
+#guard_msgs in #check WP e @ E {{ Φ }}
 /-- info: Wp.wp Stuckness.NotStuck ⊤ e Φ : PROP -/
 #guard_msgs in #check WP e {{ Φ }}
 /-- info: Wp.wp Stuckness.MaybeStuck ⊤ e Φ : PROP -/
@@ -202,17 +496,46 @@ variable (Φ : Val → PROP)
 /-- info: TotalWP.totalWp s E e Φ : PROP -/
 #guard_msgs in #check WP e @ s ; E [{ Φ }]
 /-- info: TotalWP.totalWp Stuckness.NotStuck E e Φ : PROP -/
-#guard_msgs in #check WP e @ E [{  Φ}]
+#guard_msgs in #check WP e @ E [{ Φ }]
 /-- info: TotalWP.totalWp Stuckness.NotStuck ⊤ e Φ : PROP -/
 #guard_msgs in #check WP e [{ Φ }]
 /-- info: TotalWP.totalWp Stuckness.MaybeStuck ⊤ e Φ : PROP -/
 #guard_msgs in #check WP e ? [{ Φ }]
 
+
+variable (P : PROP) (Q : PROP) (v : Nat) (s : Stuckness) [Wp PROP Expr Nat Stuckness]
+
+-- Can we do away with the `x .. y` by obtaining the identifiers directly from `RET pat`?
+
+/-- info: iprop(∀ Φ, P -∗ (▷ ∀ x y, Q → Φ (x + 1)) -∗ Wp.wp s E e Φ) : PROP -/
+#guard_msgs in #check {{{ P }}} e @ s ; E {{{ x y , RET (x+1) ; Q }}}
+/-- info: iprop(∀ Φ, P -∗ (▷ ∀ x y, Q → Φ (x + 1)) -∗ Wp.wp Stuckness.NotStuck E e Φ) : PROP -/
+#guard_msgs in #check {{{ P }}} e @ E {{{ x y , RET (x+1) ; Q }}}
+/-- info: iprop(∀ Φ, P -∗ (▷ ∀ x y, Q → Φ (x + 1)) -∗ Wp.wp Stuckness.MaybeStuck E e Φ) : PROP -/
+#guard_msgs in #check {{{ P }}} e @ E ? {{{ x y , RET (x+1) ; Q }}}
+/-- info: iprop(∀ Φ, P -∗ (▷ ∀ x y, Q → Φ (x + 1)) -∗ Wp.wp Stuckness.NotStuck ⊤ e Φ) : PROP -/
+#guard_msgs in #check {{{ P }}} e {{{ x y , RET (x+1) ; Q }}}
+/-- info: iprop(∀ Φ, P -∗ (▷ ∀ x y, Q → Φ (x + 1)) -∗ Wp.wp Stuckness.MaybeStuck ⊤ e Φ) : PROP -/
+#guard_msgs in #check {{{ P }}} e ? {{{ x y , RET (x+1) ; Q }}}
+
+#check iprop(∀ Φ, P -∗ (▷ Q → Φ 0) -∗ Wp.wp s E e Φ)
+/-- info: iprop(∀ Φ, P -∗ (▷ Q → Φ 0) -∗ Wp.wp s E e Φ) : PROP -/
+#guard_msgs in #check {{{ P }}} e @ s ; E {{{ RET 0 ; Q }}}
+/-- info: iprop(∀ Φ, P -∗ (▷ Q → Φ 0) -∗ Wp.wp Stuckness.NotStuck E e Φ) : PROP -/
+#guard_msgs in #check {{{ P }}} e @ E {{{ RET 0 ; Q }}}
+/-- info: iprop(∀ Φ, P -∗ (▷ Q → Φ 0) -∗ Wp.wp Stuckness.MaybeStuck E e Φ) : PROP -/
+#guard_msgs in #check {{{ P }}} e @ E ? {{{ RET pat ; Q }}}
+/-- info: iprop(∀ Φ, P -∗ (▷ Q → Φ 0) -∗ Wp.wp Stuckness.NotStuck ⊤ e Φ) : PROP -/
+#guard_msgs in #check {{{ P }}} e {{{ RET pat ; Q }}}
+/-- info: iprop(∀ Φ, P -∗ (▷ Q → Φ 0) -∗ Wp.wp Stuckness.MaybeStuck ⊤ e Φ) : PROP -/
+#guard_msgs in #check {{{ P }}} e ? {{{ RET pat ; Q }}}
+
+
 end testElab
 
-meta def unexpandWpPostcondInner : TSyntax `term → PrettyPrinter.UnexpandM (TSyntax `wp_postcond_inner)
-  | `(fun $v:ident => $Φ:term) => `(wp_postcond_inner|$v:ident, $Φ:term)
-  | `($Φ:term) => `(wp_postcond_inner| $Φ:term)
+meta def unexpandWpPostcondInner : TSyntax `term → PrettyPrinter.UnexpandM (TSyntax `wpPostcondInner)
+  | `(fun $v:ident => $Φ:term) => `(wpPostcondInner|$v:ident, $Φ:term)
+  | `($Φ:term) => `(wpPostcondInner| $Φ:term)
 
 open Lean in
 meta def makeWpExpr (s E e : TSyntax `term) : PrettyPrinter.UnexpandM (TSyntax `wp_expr) := do
@@ -227,16 +550,16 @@ meta def makeWpExpr (s E e : TSyntax `term) : PrettyPrinter.UnexpandM (TSyntax `
 meta def unexpanderWp : PrettyPrinter.Unexpander
   | `($_wp $s $E $e $Φ) => do
     let wp_expr ← makeWpExpr s E e
-    let wp_postcond_inner ← unexpandWpPostcondInner Φ
-    `(WP $wp_expr {{ $wp_postcond_inner }})
+    let wpPostcondInner ← unexpandWpPostcondInner Φ
+    `(WP $wp_expr {{ $wpPostcondInner }})
   | _ => throw ()
 
 @[app_unexpander TotalWP.totalWp]
 meta def unexpanderTotalWp : PrettyPrinter.Unexpander
   | `($_wp $s $E $e $Φ) => do
     let wp_expr ← makeWpExpr s E e
-    let wp_postcond_inner ← unexpandWpPostcondInner Φ
-    `(WP $wp_expr [{ $wp_postcond_inner }])
+    let wpPostcondInner ← unexpandWpPostcondInner Φ
+    `(WP $wp_expr [{ $wpPostcondInner }])
   | _ => throw ()
 
 section testUnexpand
@@ -298,3 +621,21 @@ variable (Φ : Val → PROP)
 #guard_msgs in #check WP e ? [{ Φ }]
 
 end testUnexpand
+
+/-
+Notations used in Rocq
+For Texan triples, more of the same
+
+{{{ P }}} e @ s ; E {{{  RET pat ; Q }}}
+{{{ P ]}} e @ E {{{ RET pat ; Q }}}
+{{{ P ]}} e @ E ? {{{  RET pat ; Q }}}
+{{{ P ]}} e {{{ RET pat ; Q }}}
+{{{ P ]}} e ? {{{ RET pat ; Q }}}
+
+{{{ P }}} e @ s ; E {{{ x .. y , RET pat ; Q }}}
+{{{ P }}} e @ E {{{ x .. y , RET pat ; Q }}}
+{{{ P }}} e @ E ? {{{ x .. y , RET pat ; Q }}}
+{{{ P }}} e {{{ x .. y , RET pat ; Q }}}
+{{{ P }}} e ? {{{ x .. y , RET pat ; Q }}}
+
+-/
